Add [alt], [optional], [tag], [many_until] and [some_until]
This patch provides several base combinators, and their companion
[Parser] and [StrictParser] instances.

lib/Combinators.v
@@ -38,6 +38,54 @@ Qed.
 Definition some `{Input i t} {α} (p : parser i α) `{StrictParser i t α p} : parser i (list α) :=
   cons <$> p <*> (many p).
 
+(** ** <<alt>> *)
+
+Definition alt `{Input i t} {α} (p q : parser i α) : parser i α :=
+  fun* input =>
+    match p input with
+    | inl _ => q input
+    | x => x
+    end.
+
+Infix "<|>" := alt (at level 50, left associativity) : monad_scope.
+
+Instance alt_Parser `(Input i t, !@Parser i t α _ p, !@Parser i t α _  q) : @Parser i t α _ (alt p q).
+
+Proof.
+  unfold alt.
+  constructor.
+  intros input x output equ.
+  case_eq (p input).
+  + intros e eque.
+    rewrite eque in equ.
+    now apply is_parser in equ.
+  + intros [x' output'] equ'.
+    rewrite equ' in equ.
+    inversion equ; subst.
+    now apply is_parser in equ'.
+Qed.
+
+Instance alt_Strict `(Input i t, !@StrictParser i t α _ p, !@StrictParser i t α _  q) : @StrictParser i t α _ (alt p q).
+
+Proof.
+  unfold alt.
+  constructor.
+  intros input x output equ.
+  case_eq (p input).
+  + intros e eque.
+    rewrite eque in equ.
+    now apply is_strict in equ.
+  + intros [x' output'] equ'.
+    rewrite equ' in equ.
+    inversion equ; subst.
+    now apply is_strict in equ'.
+Qed.
+
+(** ** <<optional>> *)
+
+Definition optional `{Input i t} {α} (p : parser i α) : parser i (option α) :=
+  (Some <$> p) <|> pure None.
+
 (** ** <<fail>> *)
 
 Definition fail `{Input i t} {α} (msg : string) : parser i α :=
@@ -90,3 +138,91 @@ Definition ensure `{Input i t} {α} (p : parser i α) (cond : α -> bool) : pars
 
 Definition token `{EquDec t, Input i t} (a : t) : parser i t :=
   ensure read_token (equalb a).
+
+(** ** <<tag>> *)
+
+Fixpoint tag `{EquDec t, Input i t} (x : list t) : parser i unit :=
+  match x with
+  | x :: rst => do token x *> tag rst end
+  | [] => pure tt
+  end.
+
+Instance tag_parser `(EquDec t, Input i t) (l : list t) : Parser (tag l).
+
+Proof.
+  induction l; typeclasses eauto.
+Qed.
+
+Definition tag' `{EquDec t, Input i t} (x : list t) : parser i (list t) :=
+  tag x *> pure x.
+
+(** ** <<many_until>> *)
+
+Function many_until_aux (a b i t : Type) (I : Input i t)
+    (p : parser i a) (H : StrictParser p) (q : parser i b)
+    (input : i) (acc : list a) {measure length input}
+  : error_stack + (list a * i) :=
+  match q input with
+  | inl _ => match p input with
+             | inl _ => inl ["p failed before q could succeed"%string]
+             | inr (x, output) => many_until_aux a b i t I p H q output (x :: acc)
+             end
+  | inr (_, output) => inr (rev acc, output)
+  end.
+
+Proof.
+  intros a b i t I p H q input acc e eque res x output equr equ.
+  now apply is_strict in equ.
+Defined.
+
+Definition many_until {a b} `{Input i t} (p : parser i a) `{StrictParser i t a p}
+    (q : parser i b)
+  : parser i (list a) :=
+  fun input => many_until_aux a b i t _ p _ q input [].
+
+Instance many_until_parser `(Input i t, !StrictParser (p : parser i a), !Parser (q : parser i b))
+  : Parser (many_until p q).
+
+Proof.
+  constructor.
+  intros input x output equ.
+  unfold many_until in *.
+  functional induction (many_until_aux a b i t _ p _ q input []).
+  + discriminate.
+  + destruct many_until_aux.
+    ++ discriminate.
+    ++ destruct p0 as [y output'].
+       inversion equ; subst.
+       transitivity (length output0).
+       +++ now apply IHs.
+       +++ now apply is_parser in e0.
+  + inversion equ; subst.
+    now apply is_parser in e.
+Qed.
+
+Instance many_until_strict `(Input i t, !StrictParser (p : parser i a), !StrictParser (q : parser i b))
+  : StrictParser (many_until p q).
+
+Proof.
+  constructor.
+  intros input x output equ.
+  unfold many_until in *.
+  functional induction (many_until_aux a b i t _ p _ q input []).
+  + discriminate.
+  + destruct many_until_aux.
+    ++ discriminate.
+    ++ destruct p0 as [y output'].
+       inversion equ; subst.
+       transitivity (length output0).
+       +++ now apply IHs.
+       +++ now apply is_strict in e0.
+  + inversion equ; subst.
+    now apply is_strict in e.
+Qed.
+
+(** ** <<some_until>> *)
+
+Definition some_until {a b} `{Input i t} (p : parser i a) `{StrictParser i t a p}
+    (q : parser i b)
+  : parser i (list a) :=
+  cons <$> p <*> many_until p q.
